compiler/proof_vec/jasmin_model.ec
@@ -1,752 +1,9 @@
 (* -------------------------------------------------------------------- *)
-require import AllCore BitEncoding IntDiv SmtMap Ring List StdOrder.
+require import AllCore BitEncoding IntDiv SmtMap Ring List StdOrder Bool.
 (*---*) import CoreMap Map Ring.IntID IntOrder.
-
-(* -------------------------------------------------------------------- *)
-lemma powS_minus (x p:int) : 0 < p => x ^ p  = x * x ^ (p-1).
-proof. smt (powS). qed.
-
-hint simplify pow_le0.
-hint simplify powS_minus@1.
-
-lemma pow2_1 : 2^1 = 2   by [].
-lemma pow2_2 : 2^2 = 4   by [].
-lemma pow2_3 : 2^3 = 8   by [].
-lemma pow2_4 : 2^4 = 16  by [].
-lemma pow2_5 : 2^5 = 32  by [].
-lemma pow2_6 : 2^6 = 64  by [].
-lemma pow2_7 : 2^7 = 128 by [].
-lemma pow2_8 : 2^8 = 256 by [].
-lemma pow2_16 : 2^16 = 65536 by [].
-lemma pow2_32 : 2 ^ 32 = 4294967296 by [].
-lemma pow2_64 : 2 ^ 64 = 18446744073709551616 by [].
-lemma pow2_128 : 2 ^ 128 = 340282366920938463463374607431768211456 by [].
-
-hint simplify
-  (pow2_1, pow2_2, pow2_3, pow2_4, pow2_5, pow2_6, pow2_7, pow2_8, pow2_16, pow2_32, pow2_64, pow2_128)@0.
-
-(* -------------------------------------------------------------------- *)
-lemma iotaS_minus :
-  forall (i n : int), 0 < n => iota_ i n = i :: iota_ (i + 1) (n - 1).
-proof. smt (iotaS). qed.
-
-hint simplify (iota0, iotaS_minus)@0.
-
-(* -------------------------------------------------------------------- *)
-abstract theory W.
-type t.
-
-op size : { int | 0 < size } as size_gt0.
-
-lemma size_ge0 : 0 <= size.
-proof. by apply/ltrW/size_gt0. qed.
-
-hint exact : size_gt0 size_ge0.
-
-op of_int : int -> t.
-op to_uint : t -> int.
-
-abbrev modulus = 2 ^ size.
-
-lemma modulus_ge2 : 2 <= modulus.
-proof.
-  rewrite powS_minus ?size_gt0; smt (size_gt0 powPos).
-qed.
-
-op to_sint (w:t) : int = 
- let i = to_uint w in
-  if 2^(size - 1) <= i then i - modulus
-  else i
-  axiomatized by to_sintE.
-
-op mk   : bool list -> t.
-op repr : t -> bool list.
-
-op "_.[_]" (w : t) (i : int) =
-  nth false (repr w) i.
-
-lemma getE (w : t) (i : int) : w.[i] = nth false (repr w) i.
-proof. by []. qed.
-
-abbrev modulus = 2 ^ size.
-
-lemma ge0_modulus : 0 <= modulus.
-proof.
-elim/intind: size size_ge0 => // i ge0_i ih.
-by rewrite powS // mulr_ge0.
-qed.
-
-hint exact : ge0_modulus.
-
-op normed (x : bool list) = size x = size.
-
-lemma normedP (w : bool list) :
-  normed w <=> size w = size.
-proof. by []. qed.
-
-op norm (x : bool list) =
-  take size x ++ nseq (max 0 (size - size x)) false.
-
-axiom repr_normed (w : t) : normed (repr w).
-
-lemma size_repr (w : t) : size (repr w) = size.
-proof. by apply/repr_normed. qed.
-
-lemma norm_normed (w : bool list) : normed w => norm w = w.
-proof.
-move/normedP=> sz_w; rewrite /norm sz_w subrr nseq0 cats0.
-by rewrite take_oversize // sz_w.
-qed.
-
-lemma size_norm (x : bool list) : size (norm x) = size.
-proof.
-rewrite /norm size_cat size_take // maxC /max subr_lt0.
-case: (size < size x) => h; first by rewrite nseq0.
-by rewrite size_nseq maxC /max subr_lt0 h /= addrCA subrr.
-qed.
-
-axiom mkK   x : mk (repr x) = x.
-axiom reprK x : repr (mk x) = norm x.
-
-axiom of_uintK (x : int) : to_uint (of_int x) = x %% modulus.
-axiom to_uintK : cancel to_uint of_int.
-axiom to_uint_cmp (x : t) : 0 <= to_uint x < modulus.
-
-lemma to_uintK' (x : t) : of_uint (to_uint x) = x.
-
-proof. by apply to_uintK. qed.
-
-hint simplify (of_uintK, to_uintK')@1.
-
-lemma of_sintK (x:int) : 
-   to_sint (of_int x) = 
-      if 2^(size -1) <= x %% modulus then (x %% modulus) - modulus
-      else x %% modulus.
-proof. by rewrite to_sintE of_uintK. qed.
-
-lemma to_uint_mod (x : t) : to_uint x %% modulus = to_uint x.
-proof. by rewrite modz_small // ger0_norm // to_uint_cmp. qed.
-
-lemma of_uint_mod (x : int) : of_uint (x %% modulus) = of_uint x.
-proof. by apply/(can_inj _ _ to_uintK) => /=; rewrite modz_mod. qed.
-
-lemma word_modeqP (x y : t) :
-  to_uint x %% modulus = to_uint y %% modulus => x = y.
-proof.
-move=> eq_mod; rewrite -(to_uintK x) -(to_uint_mod x).
-by rewrite eq_mod to_uint_mod.
-qed.
-
-op blift1 (f : bool -> bool) (w : t) =
-  mk (map f (repr w)).
-
-op blift2 (f : bool -> bool -> bool) (w1 w2 : t) =
-  mk (map (fun b : _ * _ => f b.`1 b.`2) (zip (repr w1) (repr w2))).
-
-op ilift1 (f : int -> int) (w : t) =
-  of_int (f (to_uint w)).
-
-op ilift2 (f : int -> int -> int) (w1 w2 : t) =
-  of_int (f (to_uint w1) (to_uint w2)).
-
-lemma get_default (w : t) (i : int) :
-  size <= i => w.[i] = false.
-proof. by move=> gt; rewrite getE nth_default // size_repr. qed.
-
-lemma get_neg (w : t) (i : int) : i < 0 => w.[i] = false.
-proof. by move=> lt0; rewrite getE nth_neg. qed.
-
-lemma mk_seqE (w : bool list) (i : int) :
-  (mk w).[i] = (0 <= i < size /\ nth false w i).
-proof.
-rewrite getE reprK; case: (0 <= i) => /=; last first.
-+ by move=> /ltrNge gt0_i; rewrite nth_neg.
-move=> ge0_i; case: (i < size) => /=; last first.
-+ by move=> /lerNgt ge_i_sz; rewrite nth_default ?size_norm.
-move=> gt_i_sz; rewrite -{2}(cat_take_drop size w) /norm.
-rewrite !nth_cat; case: (i < size (take size w)) => //.
-move=> /lerNgt h; rewrite nth_nseq_if if_same; apply/eq_sym.
-case: (size w <= size) => [ge_wsz|]; first by rewrite drop_oversize.
-move=> /ltrNge lt_szw; move: h; rewrite size_takel.
-+ by rewrite size_ge0 /= ltzW.
-+ by move/(ltr_le_trans _ _ _ gt_i_sz).
-qed.
-
-lemma blift1E (f : bool -> bool) (w : t) (i : int) :
-  (blift1 f w).[i] = (0 <= i < size /\ f w.[i]).
-proof.
-rewrite mk_seqE; apply/eq_iff/andb_id2l => h.
-by rewrite getE; apply/nth_map; rewrite size_repr.
-qed.
-
-lemma blift2E (f : bool -> bool -> bool) (w1 w2: t) (i : int) :
-  (blift2 f w1 w2).[i] = (0 <= i < size /\ f w1.[i] w2.[i]).
-proof.
-rewrite mk_seqE; apply/eq_iff/andb_id2l => h.
-rewrite !getE (nth_map (false, false)).
-+ by rewrite size_zip !size_repr.
-by rewrite nth_zip ?size_repr.
-qed. 
-
-op zeros = mk (nseq size false) axiomatized by zerosE.
-op ones  = mk (nseq size true ) axiomatized by onesE.
-
-op zerow = of_uint 0 axiomatized by zerowE.
-op ( + ) = ilift2 Int.( + ) axiomatized by addE.
-op ([-]) = ilift1 Int.([-]) axiomatized by oppE.
-op ( * ) = ilift2 Int.( * ) axiomatized by mulE.
-abbrev (-) (x y:t) = x + (-y).
-
-op (\udiv) : t -> t -> t.
-op (\umod) : t -> t -> t.
-
-op (\sdiv) : t -> t -> t.
-op (\smod) : t -> t -> t.
-
-op (`&`) = blift2 (/\) axiomatized by andE.
-op (`|`) = blift2 (\/) axiomatized by orE.
-op (`^`) = blift2 Logic.(^) axiomatized by xorE.
-
-(* FIXME : check extraction *)
-op (\sle) (x y : t) = (to_sint x) <= (to_sint y) axiomatized by wsleE.
-op (\slt) (x y : t) = (to_sint x) <  (to_sint y) axiomatized by wsltE.
- 
-op (\ule) (x y : t) = (to_uint x) <= (to_uint y) axiomatized by wuleE.
-op (\ult) (x y : t) = (to_uint x) <  (to_uint y) axiomatized by wultE.
-
-op addc : t -> t -> bool -> bool * t.
-op mulu : t -> t -> t * t.
-
-(* The type word is a ring *)
-
-op zero = of_int 0.
-op one  = of_int 1.
-
-op (^) (x:t) (p:int) = fold (( * ) x) one p
-  axiomatized by powE.
-
-lemma pow0 (x:t) : x ^ 0 = one.
-proof. by rewrite powE fold0. qed.
-
-lemma powS p x: 0 <= p => x ^ (p+1) = x * x ^ p.
-proof. by move=> ge0_p; rewrite !powE foldS. qed.
-
-lemma to_uint_small i : 0 <= i < modulus => to_uint (of_int i) = i.
-proof. move=> h; rewrite of_uintK modz_small; smt (). qed.
-hint simplify to_uint_small@0.
-
-lemma to_uint0 : to_uint zero = 0.
-proof. by rewrite /zero /=. qed.
-
-lemma to_uint1 : to_uint one = 1.
-proof. rewrite /one to_uint_small; smt (modulus_ge2). qed.
-
-lemma oner_neq0 : one <> zero.
-proof.
-  rewrite /one /zero; apply /negP => heq.
-  have := of_uintK 1. rewrite heq of_uintK mod0z.
-  rewrite modz_small //;smt (modulus_ge2).
-qed.
-
-lemma addr0 (x:t) : x + zero = x.
-proof. by rewrite addE /ilift2 to_uint0 addz0 to_uintK. qed.
-
-instance ring with t
-  op rzero = W.zero
-  op rone  = W.one
-  op add   = W.( + )
-  op opp   = W.([-])
-  op mul   = W.( * )
-  op expr  = W.( ^ )
-  op ofint = W.of_int 
-
-  proof oner_neq0 by apply oner_neq0
-  proof addr0     by smt (addr0)
-  proof addrA     by admit
-  proof addrC     by admit
-  proof addrN     by admit
-  proof mulr1     by admit
-  proof mulrA     by admit
-  proof mulrC     by admit
-  proof mulrDl    by admit
-  proof expr0     by admit
-  proof exprS     by admit
-  proof ofint0    by admit
-  proof ofint1    by admit
-  proof ofintS    by admit
-  proof ofintN    by admit.
-
-
-op (`>>>`) (x : t) (i : int) =
-  mk (mkseq (fun j => x.[j + (i %% size)]) size)
-  axiomatized by wlsrE.
-
-op (`<<<`) (x : t) (i : int) =
-  mk (mkseq (fun j => x.[j - (i %% size)]) size)
-  axiomatized by wlslE.
-
-
-lemma bandE (w1 w2 : t) (i : int) :
-  0 <= i < size => (w1 `&` w2).[i] = (w1.[i] /\ w2.[i]).
-proof. by move=> szok; rewrite andE blift2E szok. qed.
-
-lemma borE (w1 w2 : t) (i : int) :
-  0 <= i < size => (w1 `|` w2).[i] = (w1.[i] \/ w2.[i]).
-proof. by move=> szok; rewrite orE blift2E szok. qed.
-
-lemma bxorE (w1 w2 : t) (i : int) :
-  0 <= i < size => (w1 `^` w2).[i] = (w1.[i] ^ w2.[i]).
-proof. by move=> szok; rewrite xorE blift2E szok. qed.
-
-axiom xor_zero_l x : of_int 0 `^` x = x.
-axiom xor_zero_r x : x `^` of_int 0 = x.
-
-hint simplify (xor_zero_l, xor_zero_r).
-
-op slice (i : int) (n : int) (w : t) =
-  take n (drop i (repr w))
-  axiomatized by sliceE.
-
-lemma to_uint0 : to_uint zerow = 0.
-proof. by rewrite zerowE /= mod0z. qed.
-
-hint simplify to_uint0.
-
-lemma of_uintD (x y : int) : of_uint (x + y) = of_uint x + of_uint y.
-proof.
-rewrite addE /ilift2 /=; apply/word_modeqP=> /=.
-by rewrite !modz_mod !(modzDml, modzDmr).
-qed.
-
-lemma to_uintD (x y : t) : to_uint (x + y) = (to_uint x + to_uint y) %% modulus.
-proof. by rewrite addE /ilift2. qed.
+require export Jasmin_utils Jasmin_array Jasmin_word Jasmin_memory.
 
 (*
-clone export ComRing with type t <- t,
-  op zeror <- zerow,
-  op ( + ) <- ( + ),
-  op [ - ] <- [ - ],
-  op ( * ) <- ( * )
-
-  proof *.
-
-realize add0r.
-proof. by move=> x; rewrite addE /ilift2. qed.
-
-realize addrC.
-proof. by move=> x y; rewrite addE /ilift2 addrC. qed.
-
-realize addrA.
-proof.
-move=> x y z; rewrite addE /ilift2 !to_uintD -of_uint_mod modzDmr.
-by rewrite -(of_uint_mod (_ + to_uint z)) modzDml addrA.
-qed.
-*)
-end W.
-
-(* -------------------------------------------------------------------- *)
-(* FIXME shift should be done modulo the size                           *)
-theory W8.
-  clone include W with op size = 8.
-
-  op (`>>`) (w1 w2 : W8.t) = w1 `>>>` to_uint w2.
-  op (`<<`) (w1 w2 : W8.t) = w1 `<<<` to_uint w2.
-end W8.
-export W8. 
-
-(* -------------------------------------------------------------------- *)
-theory W16.
-  clone include W with op size = 16.
-
-  op (`>>`) (w1 w2 : W16.t) = w1 `>>>` to_uint w2.
-  op (`<<`) (w1 w2 : W16.t) = w1 `<<<` to_uint w2.
-end W16. 
-export W16. 
-
-(* -------------------------------------------------------------------- *)
-theory W32.
-  clone include W with op size = 32.
-
-  op (`>>`) (w1 : W32.t) (w2 : W8.t) = w1 `>>>` to_uint w2.
-  op (`<<`) (w1 : W32.t) (w2 : W8.t) = w1 `<<<` to_uint w2.
-end W32.
-export W32. 
-
-(* -------------------------------------------------------------------- *)
-theory W64.
-  clone include W with op size = 64.
-
-  op (`>>`) (w1 : W64.t) (w2 : W8.t) = w1 `>>>` to_uint w2.
-  op (`<<`) (w1 : W64.t) (w2 : W8.t) = w1 `<<<` to_uint w2.
-end W64. 
-export W64. 
-
-(* -------------------------------------------------------------------- *)
-theory W128.
-  clone include W with op size = 128.
-
-  op (`>>`) (w1 : W128.t) (w2 : W8.t) = w1 `>>>` to_uint w2.
-  op (`<<`) (w1 : W128.t) (w2 : W8.t) = w1 `<<<` to_uint w2.
-end W128. 
-export W128. 
-
-(* -------------------------------------------------------------------- *)
-theory W256.
-  clone include W with op size = 256.
-
-  op (`>>`) (w1 : W256.t) (w2 : W8.t) = w1 `>>>` to_uint w2.
-  op (`<<`) (w1 : W256.t) (w2 : W8.t) = w1 `<<<` to_uint w2.
-end W256. 
-export W256. 
-
-hint simplify (W8.to_uint_small, W16.to_uint_small, W32.to_uint_small, 
-               W64.to_uint_small, W128.to_uint_small, W256.to_uint_small)@0. 
-
-hint simplify (W8.of_uintK, W8.to_uintK')@1.
-hint simplify (W16.of_uintK, W16.to_uintK')@1.
-hint simplify (W32.of_uintK, W32.to_uintK')@1.
-hint simplify (W64.of_uintK, W64.to_uintK')@1.
-hint simplify (W128.of_uintK, W128.to_uintK')@1.
-hint simplify (W256.of_uintK, W256.to_uintK')@1.
-
-
-hint simplify (W8.xor_zero_l, W8.xor_zero_r)@0.  
-hint simplify (W16.xor_zero_l, W16.xor_zero_r)@0.  
-hint simplify (W32.xor_zero_l, W32.xor_zero_r)@0.  
-hint simplify (W64.xor_zero_l, W64.xor_zero_r)@0.  
-hint simplify (W128.xor_zero_l, W128.xor_zero_r)@0.  
-hint simplify (W256.xor_zero_l, W256.xor_zero_r)@0.  
-
-(* -------------------------------------------------------------------- *)
-op sigext_8_16  = fun x => W16.of_int  (W8.to_sint x)
-  axiomatized by sigext_8_16E.
-
-op sigext_8_32  = fun x => W32.of_int  (W8.to_sint x)
-  axiomatized by sigext_8_32E.
-
-op sigext_8_64  = fun x => W64.of_int  (W8.to_sint x)
-  axiomatized by sigext_8_64E.
-
-op sigext_8_128 = fun x => W128.of_int (W8.to_sint x)
-  axiomatized by sigext_8_128E.
-
-op sigext_8_256 = fun x => W256.of_int (W8.to_sint x)
-  axiomatized by sigext_8_256E.
-
-(* -------------------------------------------------------------------- *)
-op sigext_16_32  = fun x => W32.of_int  (W16.to_sint x)
-  axiomatized by sigext_16_32E.
-
-op sigext_16_64  = fun x => W64.of_int  (W16.to_sint x)
-  axiomatized by sigext_16_64E.
-
-op sigext_16_128 = fun x => W128.of_int (W16.to_sint x)
-  axiomatized by sigext_16_128E.
-
-op sigext_16_256 = fun x => W256.of_int (W16.to_sint x)
-  axiomatized by sigext_16_256E.
-
-(* -------------------------------------------------------------------- *)
-op sigext_32_64  = fun x => W64.of_int  (W32.to_sint x)
-  axiomatized by sigext_32_64E.
-
-op sigext_32_128 = fun x => W128.of_int (W32.to_sint x)
-  axiomatized by sigext_32_128E.
-
-op sigext_32_256 = fun x => W256.of_int (W32.to_sint x)
-  axiomatized by sigext_32_256E.
-
-(* -------------------------------------------------------------------- *)
-op sigext_64_128 = fun x => W128.of_int (W64.to_sint x)
-  axiomatized by sigext_64_128E.
-
-op sigext_64_256 = fun x => W256.of_int (W64.to_sint x)
-  axiomatized by sigext_64_256E.
-
-(* -------------------------------------------------------------------- *)
-op sigext_128_256 = fun x => W256.of_int (W128.to_sint x)
-  axiomatized by sigext_128_256E.
-
-(* -------------------------------------------------------------------- *)
-op zeroext_8_16  = fun x => W16.of_int  (W8.to_uint x)
-  axiomatized by zeroext_8_16E.
-
-op zeroext_8_32  = fun x => W32.of_int  (W8.to_uint x)
-  axiomatized by zeroext_8_32E.
-
-op zeroext_8_64  = fun x => W64.of_int  (W8.to_uint x)
-  axiomatized by zeroext_8_64E.
-
-op zeroext_8_128 = fun x => W128.of_int (W8.to_uint x)
-  axiomatized by zeroext_8_128E.
-
-op zeroext_8_256 = fun x => W256.of_int (W8.to_uint x)
-  axiomatized by zeroext_8_256E.
-
-(* -------------------------------------------------------------------- *)
-op zeroext_16_8   = fun x => W8.of_int   (W16.to_uint x)
-  axiomatized by zeroext_16_8E.
-
-op zeroext_16_32  = fun x => W32.of_int  (W16.to_uint x)
-  axiomatized by zeroext_16_32E.
-
-op zeroext_16_64  = fun x => W64.of_int  (W16.to_uint x)
-  axiomatized by zeroext_16_64E.
-
-op zeroext_16_128 = fun x => W128.of_int (W16.to_uint x)
-  axiomatized by zeroext_16_128E.
-
-op zeroext_16_256 = fun x => W256.of_int (W16.to_uint x)
-  axiomatized by zeroext_16_256E.
-
-(* -------------------------------------------------------------------- *)
-op zeroext_32_8   = fun x => W8.of_int   (W32.to_uint x)
-  axiomatized by zeroext_32_8E.
-
-op zeroext_32_16  = fun x => W16.of_int  (W32.to_uint x)
-  axiomatized by zeroext_32_16E.
-
-op zeroext_32_64  = fun x => W64.of_int  (W32.to_uint x)
-  axiomatized by zeroext_32_64E.
-
-op zeroext_32_128 = fun x => W128.of_int (W32.to_uint x)
-  axiomatized by zeroext_32_128E.
-
-op zeroext_32_256 = fun x => W256.of_int (W32.to_uint x)
-  axiomatized by zeroext_32_256E.
-
-(* -------------------------------------------------------------------- *)
-op zeroext_64_8   = fun x => W8.of_int   (W64.to_uint x)
-  axiomatized by zeroext_64_8E.
-
-op zeroext_64_16  = fun x => W16.of_int  (W64.to_uint x)
-  axiomatized by zeroext_64_16E.
-
-op zeroext_64_32  = fun x => W32.of_int  (W64.to_uint x)
-  axiomatized by zeroext_64_32E.
-
-op zeroext_64_128 = fun x => W128.of_int (W64.to_uint x)
-  axiomatized by zeroext_64_128E.
-
-op zeroext_64_256 = fun x => W256.of_int (W64.to_uint x)
-  axiomatized by zeroext_64_256E.
-
-(* -------------------------------------------------------------------- *)
-op zeroext_128_8   = fun x => W8.of_int   (W128.to_uint x)
-  axiomatized by zeroext_128_8E.
-
-op zeroext_128_16  = fun x => W16.of_int  (W128.to_uint x)
-  axiomatized by zeroext_128_16E.
-
-op zeroext_128_32  = fun x => W32.of_int  (W128.to_uint x)
-  axiomatized by zeroext_128_32E.
-
-op zeroext_128_64  = fun x => W64.of_int  (W128.to_uint x)
-  axiomatized by zeroext_128_64E.
-
-op zeroext_128_256 = fun x => W256.of_int (W128.to_uint x)
-  axiomatized by zeroext_128_256E.
-
-(* -------------------------------------------------------------------- *)
-op zeroext_256_8   = fun x => W8.of_int   (W256.to_uint x)
-  axiomatized by zeroext_256_8E.
-
-op zeroext_256_16  = fun x => W16.of_int  (W256.to_uint x)
-  axiomatized by zeroext_256_16E.
-
-op zeroext_256_32  = fun x => W32.of_int  (W256.to_uint x)
-  axiomatized by zeroext_256_32E.
-
-op zeroext_256_64  = fun x => W64.of_int  (W256.to_uint x)
-  axiomatized by zeroext_256_64E.
-
-op zeroext_256_128 = fun x => W128.of_int (W256.to_uint x)
-  axiomatized by zeroext_256_128E.
-
-(* -------------------------------------------------------------------- *)
-abbrev [-printing] u8_16  = zeroext_8_16.
-abbrev [-printing] u8_32  = zeroext_8_32.
-abbrev [-printing] u8_64  = zeroext_8_64.
-abbrev [-printing] u8_128 = zeroext_8_128.
-abbrev [-printing] u8_256 = zeroext_8_256.
-
-abbrev [-printing]  u16_8 = zeroext_16_8.
-abbrev [-printing]  u32_8 = zeroext_32_8.
-abbrev [-printing]  u64_8 = zeroext_64_8.
-abbrev [-printing] u128_8 = zeroext_128_8.
-abbrev [-printing] u256_8 = zeroext_256_8.
-
-(* -------------------------------------------------------------------- *)
-theory W8List.
-  abbrev "_.[_]" (w : W8.t list) (i : int) = nth W8.zero w i.
-end W8List.
-export W8List.
-
-(* -------------------------------------------------------------------- *)
-op unpackW16 (w : W16.t) : W8.t list =
-  map (fun i => u16_8 (w `>>>` (i * 8))) (range 0 2).
-
-op unpackW32 (w : W32.t) : W8.t list =
-  map (fun i => u32_8 (w `>>>` (i * 8))) (range 0 4).
-
-op unpackW64 (w : W64.t) : W8.t list =
-  map (fun i => u64_8 (w `>>>` (i * 8))) (range 0 8).
-
-op unpackW128 (w : W128.t) : W8.t list =
-  map (fun i => u128_8 (w `>>>` (i * 8))) (range 0 16).
-
-op unpackW256 (w : W256.t) : W8.t list =
-  map (fun i => u256_8 (w `>>>` (i * 8))) (range 0 32).
-
-(* -------------------------------------------------------------------- *)
-op packW16 (w : W8.t list) =
-      (u8_16 w.[0] `<<<` (0 * 8))
-  `^` (u8_16 w.[1] `<<<` (1 * 8)).
-
-op packW32 (w : W8.t list) =
-      (u8_32 w.[0] `<<<` (0 * 8))
-  `^` (u8_32 w.[1] `<<<` (1 * 8))
-  `^` (u8_32 w.[2] `<<<` (2 * 8))
-  `^` (u8_32 w.[3] `<<<` (3 * 8)).
-
-op packW64 (w : W8.t list) =
-      (u8_64 w.[0] `<<<` 0 * 8)
-  `^` (u8_64 w.[1] `<<<` 1 * 8)
-  `^` (u8_64 w.[2] `<<<` 2 * 8)
-  `^` (u8_64 w.[3] `<<<` 3 * 8)
-  `^` (u8_64 w.[4] `<<<` 4 * 8)
-  `^` (u8_64 w.[5] `<<<` 5 * 8)
-  `^` (u8_64 w.[6] `<<<` 6 * 8)
-  `^` (u8_64 w.[7] `<<<` 7 * 8).
-
-op packW128 (w : W8.t list) =
-      (u8_128 w.[ 0] `<<<`  0 * 8)
-  `^` (u8_128 w.[ 1] `<<<`  1 * 8)
-  `^` (u8_128 w.[ 2] `<<<`  2 * 8)
-  `^` (u8_128 w.[ 3] `<<<`  3 * 8)
-  `^` (u8_128 w.[ 4] `<<<`  4 * 8)
-  `^` (u8_128 w.[ 5] `<<<`  5 * 8)
-  `^` (u8_128 w.[ 6] `<<<`  6 * 8)
-  `^` (u8_128 w.[ 7] `<<<`  7 * 8)
-  `^` (u8_128 w.[ 8] `<<<`  8 * 8)
-  `^` (u8_128 w.[ 9] `<<<`  9 * 8)
-  `^` (u8_128 w.[10] `<<<` 10 * 8)
-  `^` (u8_128 w.[11] `<<<` 11 * 8)
-  `^` (u8_128 w.[12] `<<<` 12 * 8)
-  `^` (u8_128 w.[13] `<<<` 13 * 8)
-  `^` (u8_128 w.[14] `<<<` 14 * 8)
-  `^` (u8_128 w.[15] `<<<` 15 * 8).
-
-op packW256 (w : W8.t list) =
-      (u8_256 w.[ 0] `<<<`  0 * 8)
-  `^` (u8_256 w.[ 1] `<<<`  1 * 8)
-  `^` (u8_256 w.[ 2] `<<<`  2 * 8)
-  `^` (u8_256 w.[ 3] `<<<`  3 * 8)
-  `^` (u8_256 w.[ 4] `<<<`  4 * 8)
-  `^` (u8_256 w.[ 5] `<<<`  5 * 8)
-  `^` (u8_256 w.[ 6] `<<<`  6 * 8)
-  `^` (u8_256 w.[ 7] `<<<`  7 * 8)
-  `^` (u8_256 w.[ 8] `<<<`  8 * 8)
-  `^` (u8_256 w.[ 9] `<<<`  9 * 8)
-  `^` (u8_256 w.[10] `<<<` 10 * 8)
-  `^` (u8_256 w.[11] `<<<` 11 * 8)
-  `^` (u8_256 w.[12] `<<<` 12 * 8)
-  `^` (u8_256 w.[13] `<<<` 13 * 8)
-  `^` (u8_256 w.[14] `<<<` 14 * 8)
-  `^` (u8_256 w.[15] `<<<` 15 * 8)
-  `^` (u8_256 w.[16] `<<<` 16 * 8)
-  `^` (u8_256 w.[17] `<<<` 17 * 8)
-  `^` (u8_256 w.[18] `<<<` 18 * 8)
-  `^` (u8_256 w.[19] `<<<` 19 * 8)
-  `^` (u8_256 w.[20] `<<<` 20 * 8)
-  `^` (u8_256 w.[21] `<<<` 21 * 8)
-  `^` (u8_256 w.[22] `<<<` 22 * 8)
-  `^` (u8_256 w.[23] `<<<` 23 * 8)
-  `^` (u8_256 w.[24] `<<<` 24 * 8)
-  `^` (u8_256 w.[25] `<<<` 25 * 8)
-  `^` (u8_256 w.[26] `<<<` 26 * 8)
-  `^` (u8_256 w.[27] `<<<` 27 * 8)
-  `^` (u8_256 w.[28] `<<<` 28 * 8)
-  `^` (u8_256 w.[29] `<<<` 29 * 8)
-  `^` (u8_256 w.[30] `<<<` 30 * 8)
-  `^` (u8_256 w.[31] `<<<` 31 * 8).
-
-(* -------------------------------------------------------------------- *)
-type address = W64.t.
-
-type global_mem_t = (address, W8.t) map.
-
-op loads (m : global_mem_t) (a : address) (l : int) =
-  map (fun i => m.[a + W64.of_int i]) (range 0 l).
-
-op stores (m : global_mem_t) (a : address) (w : W8.t list) =
-  foldl (fun (m:global_mem_t) i => m.[a + W64.of_int i <- w.[i]]) m (range 0 (size w)).
-
-op loadW8   (m : global_mem_t) (a : address) = m.[a]                   axiomatized by loadW8E.
-op loadW16  (m : global_mem_t) (a : address) = packW16  (loads m a  2) axiomatized by loadW16E.
-op loadW32  (m : global_mem_t) (a : address) = packW32  (loads m a  4) axiomatized by loadW32E.
-op loadW64  (m : global_mem_t) (a : address) = packW64  (loads m a  8) axiomatized by loadW64E.
-op loadW128 (m : global_mem_t) (a : address) = packW128 (loads m a 16) axiomatized by loadW128E.
-op loadW256 (m : global_mem_t) (a : address) = packW256 (loads m a 32) axiomatized by loadW256E.
-
-op storeW8 (m : global_mem_t) (a : address) (w : W8.t) =
-  m.[a <- w]
-axiomatized by storeW8E.
-
-op storeW16 (m : global_mem_t) (a : address) (w : W16.t) =
-  stores m a (unpackW16 w)
-axiomatized by storeW16E.
-
-op storeW32 (m : global_mem_t) (a : address) (w : W32.t) =
-  stores m a (unpackW32 w)
-axiomatized by storeW32E.
-
-op storeW64 (m : global_mem_t) (a : address) (w : W64.t) =
-  stores m a (unpackW64 w)
-axiomatized by storeW64E.
-
-op storeW128 (m : global_mem_t) (a : address) (w : W128.t) =
-  stores m a (unpackW128 w)
-axiomatized by storeW128E.
-
-op storeW256 (m : global_mem_t) (a : address) (w : W256.t) =
-  stores m a (unpackW256 w)
-axiomatized by storeW256E.
-
-(* ------------------------------------------------------------------- *)
-(* Global Memory                                                       *)
-
-module Glob = {
-  var mem : global_mem_t
-}.
-
-(* -------------------------------------------------------------------- *)
-type p4u32 = W32.t * W32.t * W32.t * W32.t.
-
-op unpack_4u32 (w : W128.t) : p4u32 =
-  (W32.mk (W128.slice  0 32 w), 
-   W32.mk (W128.slice 32 32 w),
-   W32.mk (W128.slice 64 32 w),
-   W32.mk (W128.slice 96 32 w) )
-  axiomatized by unpack_4u32_E.
-
-op pack_4u32 (w : p4u32) : W128.t =
-  W128.mk (W32.repr w.`1 ++ W32.repr w.`2 ++ W32.repr w.`3 ++ W32.repr w.`4)
-  axiomatized by pack_4u32_E.
-
-axiom pack_unpack_4u32 w : pack_4u32 (unpack_4u32 w) = w.
-
-axiom unpack_pack_4u32 w : 
-  unpack_4u32 (pack_4u32 w) = w.
-
-hint simplify (pack_unpack_4u32, unpack_pack_4u32)@0.
-
-op map_4u32 (f : W32.t -> W32.t) (w : p4u32) : p4u32 =
-  (f w.`1, f w.`2, f w.`3, f w.`4).
-
-op map2_4u32 (f : W32.t -> W32.t -> W32.t) (w1 w2:p4u32) : p4u32 = 
-  (f w1.`1 w2.`1, f w1.`2 w2.`2, f w1.`3 w2.`3, f w1.`4 w2.`4).
-
 axiom VPAND_128_32 (w1 w2 : p4u32):
   (pack_4u32 w1 `&` pack_4u32 w2) = 
   pack_4u32 (map2_4u32 W32.(`&`) w1 w2).
@@ -760,17 +17,15 @@ axiom VPXOR_128_32 (w1 w2 : p4u32):
   pack_4u32 (map2_4u32 W32.(`^`) w1 w2).
 
 hint simplify (VPAND_128_32, VPOR_128_32, VPXOR_128_32)@0.
-
+*)
 (* -------------------------------------------------------------------- *)
-op x86_MOVD_32 (x : W32.t) =
-  pack_4u32 (x, W32.zero, W32.zero, W32.zero).
+abbrev x86_MOVD_32 (x : W32.t) = pack4 [x; W32.zero; W32.zero; W32.zero].
 
-(* FIXME cnt should be unsigned int mod 32 *)
 op x86_ROL_32 (x : W32.t) (cnt : W8.t) =
-  let result = rot (to_uint cnt) (repr x) in
-  let CF = last true result in
-  let OF = Logic.(^) CF (head true result) in
-  (CF, OF, W32.mk result)
+  let result = W32.rol x (to_uint cnt) in
+  let CF = result.[0] in
+  let OF = Logic.(^) CF result.[31] in
+  (CF, OF, result)
   axiomatized by x86_ROL_32_E.
 
 (* -------------------------------------------------------------------- *)
@@ -787,88 +42,42 @@ op x86_SHRD_64 :
   W64.t -> W64.t -> W8.t -> (bool * bool * bool * bool * bool * W64.t).
 
 (* -------------------------------------------------------------------- *)
-op x86_VPSLL_4u32 (w : W128.t) (cnt : W8.t) =
-  let f = fun w : W32.t => w `<<` cnt in
-  pack_4u32 (map_4u32 f (unpack_4u32 w)).
 
-op x86_VPSRL_4u32 (w : W128.t) (cnt : W8.t) =
-  let f = fun w : W32.t => w `>>` cnt in
-  pack_4u32 (map_4u32 f (unpack_4u32 w)).
+abbrev x86_VPSLL_16u8 (w : W128.t) (cnt : W8.t) = 
+  map (fun (w:W8.t) => w `<<` cnt) w.
+
+abbrev x86_VPSLL_8u16 (w : W128.t) (cnt : W8.t) = 
+  map (fun (w:W16.t) => w `<<` cnt) w.
+
+abbrev x86_VPSLL_4u32 (w : W128.t) (cnt : W8.t) = 
+  map (fun (w:W32.t) => w `<<` cnt) w.
+
+abbrev x86_VPSLL_2u64 (w : W128.t) (cnt : W8.t) = 
+  map (fun (w:W64.t) => w `<<` cnt) w.
+
+abbrev x86_VPSRL_16u8 (w : W128.t) (cnt : W8.t) = 
+  map (fun (w:W8.t) => w `>>` cnt) w.
+
+abbrev x86_VPSRL_8u16 (w : W128.t) (cnt : W8.t) = 
+  map (fun (w:W16.t) => w `>>` cnt) w.
+
+abbrev x86_VPSRL_4u32 (w : W128.t) (cnt : W8.t) = 
+  map (fun (w:W32.t) => w `>>` cnt) w.
+
+abbrev x86_VPSRL_2u64 (w : W128.t) (cnt : W8.t) = 
+  map (fun (w:W64.t) => w `>>` cnt) w.
 
 (* -------------------------------------------------------------------- *)
-type p16u8 = W8.t * W8.t * W8.t * W8.t * W8.t * W8.t * W8.t * W8.t *
-             W8.t * W8.t * W8.t * W8.t * W8.t * W8.t * W8.t * W8.t.
 
-op unpack_16u8 (w : W128.t) : p16u8 =
-  (W8.mk (W128.slice 0 8 w),
-   W8.mk (W128.slice 8 8 w),
-   W8.mk (W128.slice 16 8 w),
-   W8.mk (W128.slice 24 8 w),
-   W8.mk (W128.slice 32 8 w),
-   W8.mk (W128.slice 40 8 w),
-   W8.mk (W128.slice 48 8 w),
-   W8.mk (W128.slice 56 8 w),
-   W8.mk (W128.slice 64 8 w),
-   W8.mk (W128.slice 72 8 w),
-   W8.mk (W128.slice 80 8 w),
-   W8.mk (W128.slice 88 8 w),
-   W8.mk (W128.slice 96 8 w),
-   W8.mk (W128.slice 104 8 w),
-   W8.mk (W128.slice 112 8 w),
-   W8.mk (W128.slice 120 8 w))
-  axiomatized by unpack_16u8_E.
-
-op p16u8_l (w:p16u8) = 
-   [ w.`1; w.`2; w.`3; w.`4; w.`5; w.`6; w.`7; w.`8;
-     w.`9;  w.`10; w.`11; w.`12; w.`13; w.`14; w.`15; w.`16 ].
-
-op pack_16u8 (w : p16u8) : W128.t =
-  W128.mk (List.flatten (List.map W8.repr (p16u8_l w)))
-  axiomatized by pack_16u8_E.
-
-axiom pack_unpack_16u8 w : pack_16u8 (unpack_16u8 w) = w.
-
-axiom unpack_pack_16u8 w : 
-  unpack_16u8 (pack_16u8 w) = w.
-
-hint simplify pack_unpack_16u8.
-hint simplify unpack_pack_16u8.
-
-op map_16u8 (f : W8.t -> W8.t) (w : p16u8) : p16u8 =
-  ( f w.`1, f w.`2, f w.`3, f w.`4, f w.`5, f w.`6, f w.`7, f w.`8,
-    f w.`9, f w.`10, f w.`11, f w.`12, f w.`13, f w.`14, f w.`15, f w.`16 ).
-
-op map2_16u8 (f : W8.t -> W8.t -> W8.t) (w1 w2 : p16u8) : p16u8 =
-  ( f w1.`1  w2.`1 , 
-    f w1.`2  w2.`2 , 
-    f w1.`3  w2.`3 , 
-    f w1.`4  w2.`4 , 
-    f w1.`5  w2.`5 , 
-    f w1.`6  w2.`6 , 
-    f w1.`7  w2.`7 , 
-    f w1.`8  w2.`8 ,
-    f w1.`9  w2.`9 , 
-    f w1.`10 w2.`10, 
-    f w1.`11 w2.`11, 
-    f w1.`12 w2.`12, 
-    f w1.`13 w2.`13, 
-    f w1.`14 w2.`14, 
-    f w1.`15 w2.`15, 
-    f w1.`16 w2.`16 ).
-
-op x86_VPSHUFB_128_B (w:W8.t list) (m : W8.t) =
+op x86_VPSHUFB_128_B (w:W128.t) (m : W8.t) =
   let i = W8.to_uint m in
   if 128 <= i then W8.zero 
-  else
-    let i = i %% 16 in
-    nth W8.zero w i.
+  else w \bits8 (i %% 16).
     
 op x86_VPSHUFB_128 (w m : W128.t) : W128.t =
-  let w = p16u8_l (unpack_16u8 w) in
-  let m = unpack_16u8 m in
-  pack_16u8 (map_16u8 (x86_VPSHUFB_128_B w) m).
+  map (x86_VPSHUFB_128_B w) m.
 
-axiom VPAND_128_8 (w1 w2 : p16u8):
+(*axiom VPAND_128_8 (w1 w2 : p16u8):
   (pack_16u8 w1 `&` pack_16u8 w2) = 
   pack_16u8 (map2_16u8 W8.(`&`) w1 w2).
 
@@ -883,109 +92,55 @@ axiom VPXOR_128_8 (w1 w2 : p16u8):
 hint simplify VPAND_128_8.
 hint simplify VPOR_128_8.
 hint simplify VPXOR_128_8.
-
+*)
 (* -------------------------------------------------------------------- *)
-op x86_VPSHUFD_128_B (w : W32.t list) (m : W8.t) (i : int) : W32.t =
+op x86_VPSHUFD_128_B (w : W128.t) (m : W8.t) (i : int) : W32.t =
   let m = W8.to_uint m in
   let p = (m %/ (2^(2*i)))%%4 in
-  nth W32.zero w p.
-
-op p4u32_l (w:p4u32) = [w.`1; w.`2; w.`3; w.`4].
+  w \bits32 p.
 
 op x86_VPSHUFD_128 (w : W128.t) (m : W8.t) : W128.t =
-  let w = p4u32_l (unpack_4u32 w) in
-  pack_4u32 (x86_VPSHUFD_128_B w m 0,
-             x86_VPSHUFD_128_B w m 1,
-             x86_VPSHUFD_128_B w m 2,
-             x86_VPSHUFD_128_B w m 3).
+  pack4 (mkseq (x86_VPSHUFD_128_B w m) 4).
+
 
 (* -------------------------------------------------------------------- *)
-type p2u32 = W32.t * W32.t.
-
-op unpack_2u32 (w:W64.t) = 
-  ( W32.mk (W64.slice 0 32 w), 
-    W32.mk (W64.slice 32 32 w) )
-  axiomatized by unpack_2u32_E.
-
-op pack_2u32 (w:p2u32) = 
-  W64.mk (W32.repr w.`1 ++ W32.repr w.`2)
-  axiomatized by pack_2u32_E.
-
-axiom pack_unpack_2u32 w : pack_2u32 (unpack_2u32 w) = w.
-axiom unpack_pack_2u32 w : unpack_2u32 (pack_2u32 w) = w.
-
-hint simplify (pack_unpack_2u32, unpack_pack_2u32)@0.
 
 op mulu_64 (w1 w2 : W64.t) = 
-  let p1 = unpack_2u32 w1 in
-  let p2 = unpack_2u32 w2 in
-  pack_2u32 (W32.mulu p1.`1 p2.`1). 
+  let (p1,p2) = (W32.mulu (w1 \bits32 0) (w2 \bits32 0)) in
+  pack2 [p1; p2].
  
 (* -------------------------------------------------------------------- *)
-type p2u64 = W64.t * W64.t.
-
-op unpack_2u64 (w : W128.t) : p2u64 =
-  ( W64.mk (W128.slice 0 64 w),
-    W64.mk (W128.slice 64 64 w) )
-  axiomatized by unpack_2u64_E. 
-
-op pack_2u64 (w : p2u64) : W128.t =
-  W128.mk (W64.repr w.`1 ++ W64.repr w.`2)
-  axiomatized by pack_2u64_E. 
-
-axiom pack_unpack_2u64 w : pack_2u64 (unpack_2u64 w) = w.
-axiom unpack_pack_2u64 w : unpack_2u64 (pack_2u64 w) = w.
-
-hint simplify (pack_unpack_2u64, unpack_pack_2u64)@0.
-
-op map_2u64 (f : W64.t -> W64.t) (w : p2u64) : p2u64 =
-  (f w.`1, f w.`2).
-
-op map2_2u64 (f : W64.t -> W64.t -> W64.t) (w1 w2 : p2u64) : p2u64 =
-  (f w1.`1 w2.`1, f w1.`2 w2.`2).
 
 op x86_VPADD_2u64 (w1 : W128.t) (w2:W128.t) = 
-   pack_2u64 (map2_2u64 W64.(+) (unpack_2u64 w1) (unpack_2u64 w2)).
+   map2 W64.(+) w1 w2.
+
 
 op x86_VPEXTR_64 (w:W128.t) (i:W8.t) = 
-  let p = unpack_2u64 w in
-  if W8.to_uint i = 0 then p.`1 
-  else if W8.to_uint i = 1 then p.`2 
+  if W8.to_uint i = 0 then (w \bits64 0)
+  else if W8.to_uint i = 1 then (w \bits64 1)
   else W64.of_int 0.
 
 op x86_VPINSR_2u64 (v1:W128.t) (v2:W64.t) (i:W8.t) = 
-  let p = unpack_2u64 v1 in
-  if W8.to_uint i = 0 then pack_2u64 (v2, p.`2)
-  else if W8.to_uint i = 1 then pack_2u64 (p.`1, v2)
+  if W8.to_uint i = 0 then (pack2 [v2; v1 \bits64 1])
+  else if W8.to_uint i = 1 then (pack2 [v1 \bits64 0; v2])
   else v1.
 
 op x86_MOVD_64 (v:W64.t) = 
-  pack_2u64 (v, W64.zero). 
+  pack2 [v; W64.zero]. 
 
 op x86_VPUNPCKL_2u64 (w1 w2: W128.t) = 
-  let p1 = unpack_2u64 w1 in
-  let p2 = unpack_2u64 w2 in
-  pack_2u64 (p1.`1, p2.`1).
+  pack2 [w1 \bits64 0; w2 \bits64 0].
 
 op x86_VPUNPCKH_2u64 (w1 w2: W128.t) = 
-  let p1 = unpack_2u64 w1 in
-  let p2 = unpack_2u64 w2 in
-  pack_2u64 (p1.`2, p2.`2).
+  pack2 [w1 \bits64 1; w2 \bits64 1].
 
-op x86_VPSLL_2u64 (w:W128.t) (cnt:W8.t) = 
-  let f = fun w : W64.t => w `<<`  cnt in
-  pack_2u64 (map_2u64 f (unpack_2u64 w)).
-
-op x86_VPSRL_2u64 (w:W128.t) (cnt:W8.t) = 
-  let f = fun w : W64.t => w `>>` cnt in
-  pack_2u64 (map_2u64 f (unpack_2u64 w)).
-
-op x86_VPAND_128 = W128.(`&`).
-op x86_VPOR_128 = W128.(`|`).
+abbrev x86_VPAND_128 = W128.(`&`).
+abbrev x86_VPOR_128 = W128.(`|`).
 
 op x86_VPMULU_128 (w1 w2: W128.t) = 
-  pack_2u64 (map2_2u64 mulu_64 (unpack_2u64 w1) (unpack_2u64 w2)).
+  map2 mulu_64 w1 w2.
 
+(*
 axiom VPAND_128_64 w1 w2:
   pack_2u64 w1 `&` pack_2u64 w2 = 
   pack_2u64(w1.`1 `&` w2.`1, w1.`2 `&` w2.`2).
@@ -999,171 +154,17 @@ axiom VPXOR_128_64 w1 w2:
   pack_2u64(w1.`1 `^` w2.`1, w1.`2 `^` w2.`2).
 
 hint simplify (VPAND_128_64, VPOR_128_64, VPXOR_128_64)@0.
-
-(*-------------------------------------------------------------------- *)
-
-abstract theory Array.
-
-  op size: int.
-
-  type 'a t.
-
-  op init : 'a -> 'a t.
-
-  op "_.[_]" ['a] : 'a t -> int -> 'a.
-
-  op "_.[_<-_]" ['a] : 'a t -> int -> 'a -> 'a t.
-
-  op map ['a 'b] : ('a -> 'b) -> 'a t -> 'b t.
-
-  axiom get_setE ['a] (t:'a t) (x y:int) (a:'a) :
-    0 <= x < size => t.[x<-a].[y] = if y = x then a else t.[y].
-
-  lemma nosmt get_set_eqE (t : 'a t) x y a :
-    0 <= x < size => y = x => t.[x <- a].[y] = a.
-  proof. by move=> h1 ->; rewrite get_setE. qed.
-
-  lemma nosmt get_set_neqE (t : 'a t) x y a :
-    0 <= x < size => y <> x => t.[x <- a].[y] = t.[y].
-  proof. by move=> h1; rewrite get_setE // => ->. qed.
-
-  axiom ext_eq (t1 t2: 'a t) : 
-    (forall x, 0 <= x < size => t1.[x] = t2.[x]) => 
-    t1 = t2.
-
-  op all_eq (t1 t2: 'a t) =
-    all (fun x => t1.[x] = t2.[x]) (range 0 size).
-
-  lemma ext_eq_all (t1 t2: 'a t) : 
-    all_eq t1 t2 <=> t1 = t2.
-  proof. 
-    split.
-    + by move=> /allP h; apply ext_eq => x /mem_range; apply h. 
-    by move=> ->;apply /allP.
-  qed.
-  
-  axiom mapE (f:'a -> 'b) (t:'a t) i : 0 <= i < size => (map f t).[i] = f (t.[i]).
-
-  op is_init (t: 'a option t) = 
-    all (fun i => t.[i] <> None) (range 0 size).
-
-  hint simplify (get_set_eqE, get_set_neqE, mapE).
-end Array.
-
-clone export Array as Array0  with op size <- 0.
-clone export Array as Array1  with op size <- 1.
-clone export Array as Array2  with op size <- 2.
-clone export Array as Array3  with op size <- 3.
-clone export Array as Array4  with op size <- 4.
-clone export Array as Array5  with op size <- 5.
-clone export Array as Array6  with op size <- 6.
-clone export Array as Array7  with op size <- 7.
-clone export Array as Array8  with op size <- 8.
-clone export Array as Array9  with op size <- 9.
-clone export Array as Array10  with op size <- 10.
-clone export Array as Array11  with op size <- 11.
-clone export Array as Array12  with op size <- 12.
-clone export Array as Array13  with op size <- 13.
-clone export Array as Array14  with op size <- 14.
-clone export Array as Array15  with op size <- 15.
-clone export Array as Array16  with op size <- 16.
-clone export Array as Array17  with op size <- 17.
-clone export Array as Array18  with op size <- 18.
-clone export Array as Array19  with op size <- 19.
-clone export Array as Array20  with op size <- 20.
-clone export Array as Array21  with op size <- 21.
-clone export Array as Array22  with op size <- 22.
-clone export Array as Array23  with op size <- 23.
-clone export Array as Array24  with op size <- 24.
-clone export Array as Array25  with op size <- 25.
-clone export Array as Array26  with op size <- 26.
-clone export Array as Array27  with op size <- 27.
-clone export Array as Array28  with op size <- 28.
-clone export Array as Array29  with op size <- 29.
-
-hint simplify (Array0.get_set_eqE, Array0.get_set_neqE, Array0.mapE)@0.
-hint simplify (Array1.get_set_eqE, Array1.get_set_neqE, Array1.mapE)@0.
-hint simplify (Array2.get_set_eqE, Array2.get_set_neqE, Array2.mapE)@0.
-hint simplify (Array3.get_set_eqE, Array3.get_set_neqE, Array3.mapE)@0.
-hint simplify (Array4.get_set_eqE, Array4.get_set_neqE, Array4.mapE)@0.
-hint simplify (Array5.get_set_eqE, Array5.get_set_neqE, Array5.mapE)@0.
-hint simplify (Array6.get_set_eqE, Array6.get_set_neqE, Array6.mapE)@0.
-hint simplify (Array7.get_set_eqE, Array7.get_set_neqE, Array7.mapE)@0.
-hint simplify (Array8.get_set_eqE, Array8.get_set_neqE, Array8.mapE)@0.
-hint simplify (Array9.get_set_eqE, Array9.get_set_neqE, Array9.mapE)@0.
-hint simplify (Array10.get_set_eqE, Array10.get_set_neqE, Array10.mapE)@0.
-hint simplify (Array11.get_set_eqE, Array11.get_set_neqE, Array11.mapE)@0.
-hint simplify (Array12.get_set_eqE, Array12.get_set_neqE, Array12.mapE)@0.
-hint simplify (Array13.get_set_eqE, Array13.get_set_neqE, Array13.mapE)@0.
-hint simplify (Array14.get_set_eqE, Array14.get_set_neqE, Array14.mapE)@0.
-hint simplify (Array15.get_set_eqE, Array15.get_set_neqE, Array15.mapE)@0.
-hint simplify (Array16.get_set_eqE, Array16.get_set_neqE, Array16.mapE)@0.
-hint simplify (Array17.get_set_eqE, Array17.get_set_neqE, Array17.mapE)@0.
-hint simplify (Array18.get_set_eqE, Array18.get_set_neqE, Array18.mapE)@0.
-hint simplify (Array19.get_set_eqE, Array19.get_set_neqE, Array19.mapE)@0.
-hint simplify (Array20.get_set_eqE, Array20.get_set_neqE, Array20.mapE)@0.
-hint simplify (Array21.get_set_eqE, Array21.get_set_neqE, Array21.mapE)@0.
-hint simplify (Array22.get_set_eqE, Array22.get_set_neqE, Array22.mapE)@0.
-hint simplify (Array23.get_set_eqE, Array23.get_set_neqE, Array23.mapE)@0.
-hint simplify (Array24.get_set_eqE, Array24.get_set_neqE, Array24.mapE)@0.
-hint simplify (Array25.get_set_eqE, Array25.get_set_neqE, Array25.mapE)@0.
-hint simplify (Array26.get_set_eqE, Array26.get_set_neqE, Array26.mapE)@0.
-hint simplify (Array27.get_set_eqE, Array27.get_set_neqE, Array27.mapE)@0.
-hint simplify (Array28.get_set_eqE, Array28.get_set_neqE, Array28.mapE)@0.
-hint simplify (Array29.get_set_eqE, Array29.get_set_neqE, Array29.mapE)@0.
+*)
 
 (* ------------------------------------------------------------------- *)
 (* Leakages                                                            *)
 
 type leakage_t = [
-  | LeakExpr of W64.t list
+  | LeakAddr of address list
   | LeakCond of bool
   | LeakFor  of (int * int)
 ].
 
 type leakages_t = leakage_t list.
-
-(* ------------------------------------------------------------------- *)
-(* Safety                                                              *)
-
-op is_init (x : 'a option) = x <> None.
-op in_bound (x n:int) = 0 <= x /\ x < n.
-
-type wsize = [
-  | W8
-  | W16
-  | W32
-  | W64
-  | W128
-  | W256
-].
-
-(* FIXME : define this *)
-op is_valid (m:global_mem_t) (p:W64.t) (ws:wsize) : bool.
-
-
-axiom is_valid_store8 mem sz ptr1 ptr2 w : 
-  is_valid (storeW8 mem ptr2 w) ptr1 sz = is_valid mem ptr1 sz.
-hint simplify is_valid_store8.
-
-axiom is_valid_store16 mem sz ptr1 ptr2 w : 
-  is_valid (storeW16 mem ptr2 w) ptr1 sz = is_valid mem ptr1 sz.
-hint simplify is_valid_store16.
-
-axiom is_valid_store32 mem sz ptr1 ptr2 w : 
-  is_valid (storeW32 mem ptr2 w) ptr1 sz = is_valid mem ptr1 sz.
-hint simplify is_valid_store32.
-
-axiom is_valid_store64 mem sz ptr1 ptr2 w : 
-  is_valid (storeW64 mem ptr2 w) ptr1 sz = is_valid mem ptr1 sz.
-hint simplify is_valid_store64.
-
-axiom is_valid_store128 mem sz ptr1 ptr2 w : 
-  is_valid (storeW128 mem ptr2 w) ptr1 sz = is_valid mem ptr1 sz.
-hint simplify is_valid_store128.
-
-axiom is_valid_store256 mem sz ptr1 ptr2 w : 
-  is_valid (storeW256 mem ptr2 w) ptr1 sz = is_valid mem ptr1 sz.
-hint simplify is_valid_store256.
 
 
